Make ReductionSeq unlabeled, add proofs for mem_concat and flatten

Thesis/ReductionSeq.lean
@@ -1,6 +1,6 @@
 import Mathlib.Tactic
-import Thesis.ARS
 import Mathlib.Logic.Relation
+import Thesis.RelProps
 
 namespace Thesis
 
@@ -8,24 +8,51 @@ section reduction_seq
 
 open Relation
 
-variable {α I}
-variable (A: ARS α I)
+variable {α}
+
+section rs_def
+
+variable (r: Rel α α)
+
+private structure Step (α: Type*) where
+  start: α
+  stop: α
 
 /--
-`ReductionSeq A x y ss` represents a reduction sequence in `A`,
-taking indexed reduction steps as given in `ss` from `x` to `y`.
+`ReductionSeq r x y ss` represents a reduction sequence, taking
+reduction steps as given in `ss` from `x` to `y`.
 
 An empty reduction sequence is represented by `ReductionSeq.refl`, allowing a
 reduction from `x` to `x` in 0 steps. Using `ReductionSeq.head`, a single step
-`a ⇒[i] b` can be prepended to an existing reduction sequence.
+`r a b` can be prepended to an existing reduction sequence.
 -/
-inductive ReductionSeq: α → α → List (I × α) → Prop
+inductive ReductionSeq: α → α → List (Step α) → Prop
   | refl {x} : ReductionSeq x x []
-  | head {i x y} : A.rel i x y → ReductionSeq y z ss → ReductionSeq x z ((i, y)::ss)
+  | head {x y z ss} : r x y → ReductionSeq y z ss → ReductionSeq x z (⟨x, y⟩::ss)
 
-def ReductionSeq.elems (_: ReductionSeq A x y ss) := x :: (ss.map (·.2))
+end rs_def
 
-theorem ReductionSeq.tail (hr: ReductionSeq A x y ss) (hstep: A.rel i y z) : ReductionSeq A x z (ss ++ [(i, z)]) := by
+variable {r: Rel α α}
+
+namespace ReductionSeq
+
+/-- A reduction sequence exists iff there is a reflexive-transitive reduction step. -/
+lemma exists_iff_rel_star {x y : α}: r∗ x y ↔ ∃ss, ReductionSeq r x y ss := by
+  constructor <;> intro r
+  · induction r using ReflTransGen.head_induction_on with
+    | refl => use [], refl
+    | head step seq ih =>
+        obtain ⟨ss', hss'⟩ := ih
+        exact ⟨_, head step hss'⟩
+  · rcases r with ⟨ss, r⟩
+    induction r with
+    | refl => rfl
+    | head step seq ih =>
+      exact ReflTransGen.head step ih
+
+def elems (_: ReductionSeq r x y ss) := x :: (ss.map Step.stop)
+
+theorem tail (hr: ReductionSeq r x y ss) (hstep: r y z): ReductionSeq r x z (ss ++ [⟨y, z⟩]) := by
   induction hr with
   | refl => simp; apply head hstep; apply refl
   | head step r ih =>
@@ -33,27 +60,62 @@ theorem ReductionSeq.tail (hr: ReductionSeq A x y ss) (hstep: A.rel i y z) : Red
     apply head step
     exact ih
 
-theorem ReductionSeq.concat (h₁ : ReductionSeq A x y ss) (h₂: ReductionSeq A y z ss') : ReductionSeq A x z (ss ++ ss') := by
+theorem concat (h₁ : ReductionSeq r x y ss) (h₂: ReductionSeq r y z ss'): ReductionSeq r x z (ss ++ ss') := by
   induction h₁ with
   | refl => exact h₂
-  | head hstep hseq ih =>
+  | head hstep _ ih =>
     apply head hstep (ih h₂)
 
-/-- A reduction sequence exists iff there is a reflexive-transitive reduction. -/
-lemma ReductionSeq.exists_iff_union_rel_star {x y : α}: A.union_rel∗ x y ↔ ∃ss, ReductionSeq A x y ss := by
-  constructor <;> intro r
-  · induction r using ReflTransGen.head_induction_on with
-    | refl => use [], ReductionSeq.refl
-    | head step seq ih =>
-        obtain ⟨ss', hss'⟩ := ih
-        obtain ⟨i, hi⟩ := step
-        exact ⟨_, head hi hss'⟩
-  · rcases r with ⟨ss, r⟩
-    induction r with
-    | refl => rfl
-    | head step seq ih =>
-      exact ReflTransGen.head ⟨_, step⟩ ih
+lemma y_elem (hseq: ReductionSeq r x y ss): y ∈ hseq.elems := by
+  induction hseq with
+  | refl => simp [elems]
+  | @head x y z ss step seq ih =>
+    simp [elems] at ih ⊢
+    tauto
 
+/--
+If `a` is an element of a concatenated sequence, it must be a member of one of
+the two subsequences.
+-/
+lemma mem_concat (hseq₁: ReductionSeq r x y ss₁) (hseq₂: ReductionSeq r y z ss₂):
+    ∀x, x ∈ (hseq₁.concat hseq₂).elems ↔ (x ∈ hseq₁.elems ∨ x ∈ hseq₂.elems) := by
+  intro a
+  induction hseq₁ with
+  | refl => simp [concat, elems]
+  | @head x y z ss step seq ih =>
+    simp [concat]
+    have ih := ih hseq₂
+    have := seq.y_elem
+    simp [elems] at this ih ⊢
+    clear * -ih this
+    aesop
+
+
+/--
+A reflexive-transitive reduction sequence `a₀ ->* a₁ ->* ... ->* aₙ` can be
+'flattened' (by analogy to a nested list) to a regular reduction sequence
+`a₀ -> ... -> a₁ -> ... -> aₙ` which contains all elements of the original
+sequence.
+-/
+lemma flatten (hseq: ReductionSeq r∗ x y ss):
+    ∃ss', ∃(hseq': ReductionSeq r x y ss'), ∀a ∈ hseq.elems, a ∈ hseq'.elems := by
+  induction hseq with
+  | refl =>
+    use [], refl
+    simp [elems]
+  | @head x y z ss hstep htail ih =>
+    obtain ⟨ss₁, hseq₁⟩ := exists_iff_rel_star.mp hstep
+    obtain ⟨ss₂, hseq₂, hmem⟩ := ih
+    use (ss₁ ++ ss₂), hseq₁.concat hseq₂
+    simp [mem_concat hseq₁ hseq₂]
+    intro a ha
+    simp only [elems, List.map_cons, List.mem_cons] at ha ⊢
+    rcases ha with (rfl | rfl | ha) <;> try tauto
+    · have := hmem a (by simp [elems] at ha ⊢; tauto)
+      simp only [elems, List.mem_cons] at this
+      right; assumption
+
+end ReductionSeq
 
 end reduction_seq
 
